examples/graphviz_ex.v
@@ -9,8 +9,10 @@ Local Open Scope string_scope.
 Compute (generate_dot_behaviour_expressions "USER" vending_machine_ctx 100).
 Compute (generate_dot_behaviour_expressions "MACHINE" vending_machine_ctx 100).
 Compute (generate_dot_behaviour_expressions "SYSTEM" vending_machine_ctx 100).
+
+Compute (generate_dot_behaviour_expressions "fig2_r" fig2_r_BE 6).
 Compute (generate_dot_lts fig2_r).
-Compute ( generate_dot_IOLTS fig4_k3_IOLTS).
-Compute ( generate_dot_s_IOLTS fig6_r).
+Compute (generate_dot_IOLTS fig2_r_IOLTS).
+Compute (generate_dot_s_IOLTS fig6_r).
 *)
 Local Close Scope string_scope.
